Implementation/Lean/Cpn2mCrl2.lean
@@ -2,6 +2,7 @@ import Cpn2mCrl2.Util
 import Cpn2mCrl2.Color
 import Cpn2mCrl2.Bag
 import Cpn2mCrl2.Expr
+import Cpn2mCrl2.Typing
 import Cpn2mCrl2.Net
 import Cpn2mCrl2.Semantics
 import Cpn2mCrl2.Lpe
